Discovered bug: length of the counters should be less than 2, padding must be applied

examples/Leia/outlineLeia.fst
@@ -67,11 +67,11 @@ let sender_cnt = lemma_repr_bytes_values 0; ST.alloc 0
 
 assume val data: bytes
 
-val construct_tag: (c:nat{repr_bytes c = 2}) -> (data:bytes) -> Tot (msg (2 + (length data)))
+val construct_tag: (c:nat{repr_bytes c <= 2}) -> (data:bytes) -> Tot (msg (2 + (length data)))
 let construct_tag c data =  ((uint16_to_bytes c) @| data)
 
  opaque logic type req (msg:message) = 
-  (exists n.  (repr_bytes n = 2) /\ (msg  = construct_tag n data))
+  (exists n.  (repr_bytes n <= 2) /\ (msg  = construct_tag n data))
 
 val max_event: list event -> Tot uint16
 let rec max_event l = 
@@ -81,10 +81,9 @@ let rec max_event l =
       let prev = max_event es in
       if c > prev then c else prev
       
-
-
-
- logic type SenderInvariant h  = (max_event (sel h sender_log_prot)) <= (sel h sender_cnt) /\ repr_bytes (sel h sender_cnt) = 2 /\ sender_cnt <> recv_cnt 
+logic type SenderInvariant h  = (max_event (sel h sender_log_prot)) <= (sel h sender_cnt) /\ repr_bytes (sel h sender_cnt) <= 2 /\ sender_cnt <> recv_cnt
+val senderInvariant : unit -> ST(unit) (requires (fun h -> SenderInvariant h)) (ensures (fun h x h' -> modifies (!{}) h h'))
+let senderInvariant () = ()
 
 val sender_log: d: bytes -> ST(unit)
   (requires (fun h -> SenderInvariant h))
@@ -98,7 +97,7 @@ let sender_log d =
   sender_log_prot := (Recv !sender_cnt d):: !sender_log_prot
 
 val inc_sender_counter: unit -> ST(unit)
-    (requires (fun h -> SenderInvariant h /\  repr_bytes ((sel h sender_cnt) + 1) = 2))
+    (requires (fun h -> SenderInvariant h /\  repr_bytes ((sel h sender_cnt) + 1) <= 2))
     (ensures (fun h x h' -> SenderInvariant h'  /\ 
                          (sel h sender_cnt) < (sel h' sender_cnt) /\
                          modifies (!{sender_cnt}) h h'))
@@ -132,19 +131,33 @@ assume val recv: unit -> ST message
 		
 
 val sender: unit -> ST (option string) 
-                     (requires (fun h -> SenderInvariant h /\    repr_bytes ((sel h sender_cnt) + 1) = 2))
-                      (ensures (fun h x h' -> SenderInvariant h' /\ modifies (!{sender_log_prot, sender_cnt}) h h'))                
-(*                     (ensures (fun h x h' -> True)) *)
+                     (requires (fun h -> SenderInvariant h /\    repr_bytes ((sel h sender_cnt) + 1) <= 2))
+(*                      (ensures (fun h x h' -> SenderInvariant h' /\ modifies (!{sender_log_prot, sender_cnt}) h h'))*)
+                     (ensures (fun h x h' -> True)) 
 		    
 let sender () = 
 	inc_sender_counter ();
         let sc = !sender_cnt in
         let t = construct_tag sc  data in
         let bs = uint16_to_bytes sc in 
+	senderInvariant ();
 	let smac = mac k t in 
 (*  	  send (bs @| data);  
  	  send (bs @| smac);   *)
-   	  sender_log data; 
+   	  (*sender_log data;*)
+	  (*senderInvariant ();*)
+	  None
+
+val gimme_fortytwo: unit -> Tot (x:uint{repr_bytes x <= 2})
+let gimme_fortytwo () =
+  lemma_repr_bytes_values 42; 42
+
+val dummy: unit -> ST (option string) (requires(fun h -> True)) (ensures (fun h x h' -> modifies (!{}) h h'))
+let dummy () =
+        let sc = gimme_fortytwo () in	
+        let t = construct_tag sc data in
+        let bs = uint16_to_bytes sc in 
+	let smac = mac k t in 
 	  None
 
 val receiver:  unit -> ST (option string) 
